Done with full implies partial

fullImpliesPartial.v
@@ -1,55 +1,56 @@
 Require Export stepPreservesRewind.  
   
 (*AheadOf H t1 t2: t2 is in t1's future with respect to heap H*)
-Inductive AheadOf H : thread -> thread -> Prop :=
-|noTXAheadOf : forall e, AheadOf H (None, nil, e) (None, nil, e)
+Inductive AheadOf H C : thread -> thread -> Prop :=
+|noTXAheadOf : forall e, AheadOf H C (None, nil, e) (None, nil, e)
 |inTXAheadOf : forall S e0 L L' e e', 
-                 replay H (Some(S,e0),L,e) (Some(S,e0),L',e') ->
-                 AheadOf H (Some(S,e0),L,e) (Some(S,e0),L',e').
+                 replay H C (Some(S,e0),L,e) (Some(S,e0),L',e') ->
+                 AheadOf H C (Some(S,e0),L,e) (Some(S,e0),L',e').
 
 (*Generalizes the previous relation to thread pools*)
-Inductive poolAheadOf H : pool -> pool -> Prop := 
-|SingleAheadOf : forall t t', AheadOf H t t' -> poolAheadOf H (Single t) (Single t')
+Inductive poolAheadOf H C : pool -> pool -> Prop := 
+|SingleAheadOf : forall t t', AheadOf H C t t' -> poolAheadOf H C (Single t) (Single t')
 |ParAheadOf : forall T1 T2 T1' T2', 
-           poolAheadOf H T1 T1' -> poolAheadOf H T2 T2' -> 
-           poolAheadOf H (Par T1 T2) (Par T1' T2'). 
+           poolAheadOf H C T1 T1' -> poolAheadOf H C T2 T2' -> 
+           poolAheadOf H C (Par T1 T2) (Par T1' T2'). 
+
 
 (*
  * If we can replay from one state to another and the first state is
  * invalid, then the second one must be too
  *)
-Theorem replayInvalid : forall H S e0 L e L' e' S' eA LA, 
-                          replay H (Some(S,e0),L,e) (Some(S,e0),L',e') ->
-                          validate S L H S' (abort eA LA) ->
-                          exists eA' LA', validate S L' H S' (abort eA' LA').
+Theorem replayInvalid : forall H S e0 L C e L' e' eA LA, 
+                          replay H C (Some(S,e0),L,e) (Some(S,e0),L',e') ->
+                          validate L H (abort eA LA) ->
+                          exists eA' LA', validate L' H (abort eA' LA').
 Proof.
   intros. dependent induction H0; eauto. 
   {inv H0; eauto. 
-   {assert(validate S (readItem l E v::L) H S' (abort eA LA)).
+   {assert(validate (readItem l E v::L) H (abort eA LA)).
     eapply validateAbortPropogate; eauto. eapply IHreplay in H0; eauto. }
-   {assert(validate S (readItem l E v::L) H S' (abort eA LA)).
+   {assert(validate (readItem l E v::L) H (abort eA LA)).
     eapply validateAbortPropogate; eauto. eapply IHreplay in H0; eauto. }
-   {assert(validate S (writeItem l v::L) H S' (abort eA LA)).
+   {assert(validate (writeItem l v::L) H (abort eA LA)).
     eapply validateAbortPropogate; eauto. eapply IHreplay in H0; eauto. }
   }
 Qed. 
 
 (*
- * If we can rewind/replay from one state to another and the final state is invalid,
- * then it must also be possible to rewind/replay to the portion that is still
- * valid as determined by validate 
+ * If we can rewind/replay from one state to another and the final state 
+ * is invalid, then it must also be possible to rewind/replay to the 
+ * portion that is still valid as determined by validate 
  *)         
-Theorem rewindValidPortion : forall S L H S' e' L' e0 e, 
-                               rewind H (Some(S,e0),nil,e0) (Some(S,e0),L,e) ->
-                               validate S L H S' (abort e' L') ->
-                               rewind H (Some(S,e0),nil,e0) (Some(S,e0),L',e').
+Theorem rewindValidPortion : forall S L H C e' L' e0 e, 
+                               rewind H C (Some(S,e0),nil,e0) (Some(S,e0),L,e) ->
+                               validate L H (abort e' L') ->
+                               rewind H C (Some(S,e0),nil,e0) (Some(S,e0),L',e').
 Proof.
   intros. dependent induction H0. 
   {inv H1. }
   {inv H1; eauto. 
    {inv H2. 
     {eapply IHrewind; eauto. }
-    {lookupSame. omega. }
+    {transEq. invertEq. exfalso; auto. }
    }
    {inv H2. 
     {eapply IHrewind; eauto. }
@@ -59,139 +60,251 @@ Proof.
   }
 Qed. 
 
-(**
- * AheadOf holds under an extended heap if everything in the extension has a 
- * timestamp greater tan the transactions read version
- *)
-Theorem AheadOfExtension : forall H H' S t e0 L e C, 
-                      AheadOf H t (Some(S,e0),L,e) -> S < C ->
-                      Forall (fun x : location * term * stamp => getStamp x = C) H' ->
-                      AheadOf (H'++H) t (Some(S,e0),L,e).
-Proof.
-  intros. inv H0. 
-  econstructor. eapply replayHeapExtension; eauto.  
-Qed. 
-
-(*generalize to thread pools*)
-Theorem poolAheadOfExtension : forall H H' T1 T2 C,
-                    poolAheadOf H T1 T2 -> 
-                    Forall (fun x : location * term * stamp => getStamp x = C) H' ->
-                    poolRewind C H T2 ->
-                    poolAheadOf (H'++H) T1 T2.
-Proof.
-  intros. induction H0. 
-  {constructor. inv H2. 
-   {inv H0. constructor. }
-   {eapply AheadOfExtension; eauto. }
-  }
-  {inv H2. constructor; auto. } 
-Qed. 
-
-(*
-Ltac invertEq :=
-  match goal with
-      |H:?x = ?y |- _ => solve[inv H]
-  end. 
-*)
 
 (*if the beginning of a replay aborts, then so does the endpoint*)
 Theorem abortReplay : forall S L H C L' e' e'' L'' e e0, 
-                        replay H (Some(S,e0),L,e) (Some(S,e0),L',e') ->
-                        validate S L H C (abort e'' L'') -> 
-                        validate S L' H C (abort e'' L''). 
+                        replay H C (Some(S,e0),L,e) (Some(S,e0),L',e') ->
+                        validate L H (abort e'' L'') -> 
+                        validate L' H (abort e'' L''). 
 Proof.
   intros. dependent induction H0; auto.
   inv H0; eapply IHreplay; eauto; eapply validateAbortPropogate; eauto. 
 Qed. 
 
-(*partial abort can simulate full abort*)
-Theorem fullImpliesPartial : forall C H T C' H' T' PT, 
-                               f_step C H T C' H' T' -> poolAheadOf H T PT ->
-                               poolRewind C H PT -> 
-                               exists PT', p_multistep C H PT C' H' PT' /\
-                                           poolAheadOf H' T' PT'.
+Theorem AheadOfAlloc : forall v C H T T' l,
+    poolAheadOf H C T T' -> H l = None ->
+    poolAheadOf (update H l v) C T T'. 
 Proof.
-  intros. generalize dependent PT. induction H0; intros. 
-  {inv H1. inv H4. 
-   {inv H0; exfalso; apply H7; auto. }
-   {inv H1. 
-    {econstructor. split. eapply p_multi_step. eapply p_transStep. 
-     eauto. constructor. constructor. inv H0; repeat constructor. }
-    {econstructor. split. constructor. constructor. Hint Constructors AheadOf.
-     inv H0; inv H3; decompSame; invertEq; repeat lookupSame; auto. omega. }
-   }
-  } 
-  {eapply f_stampHeapMonotonic in H0. invertHyp. inv H1. eapply IHf_step in H6. 
-   invertHyp. econstructor. split. eapply p_multi_L. eauto. constructor. auto.
-   inv H2. eapply poolAheadOfExtension; eauto. inv H2. auto. }
-  {eapply f_stampHeapMonotonic in H0. invertHyp. inv H1. eapply IHf_step in H8. 
-   invertHyp. econstructor. split. eapply p_multi_R. eauto. constructor. inv H2. 
-   eapply poolAheadOfExtension; eauto. auto. auto. inv H2. auto. 
+  intros. induction H0.
+  {inv H0.
+   {repeat constructor. }
+   {rewrite <- rewindIFFReplay in H2. eapply rewindAllocSingle in H2; eauto.
+    constructor. constructor. rewrite <- rewindIFFReplay. eauto. }
   }
-  {inv H1. inv H4. econstructor. split. eapply p_multi_step.
-   eapply p_forkStep; eauto. constructor. repeat constructor. }
-  {inv H5. inv H8. inv H12. 
-   {econstructor. split. eapply p_multi_step. eapply p_eagerAbort; eauto.
-    constructor. repeat constructor. inv H6. rewrite <- rewindIFFReplay.
-    assert(rewind H (Some(S,e0),nil,e0) (Some(S,e0),(readItem l E v :: L'0), fill E v)). 
-    econstructor. eauto. eapply r_readStepInvalid; eauto. omega. copy H2.
-    eapply validateValidate in H2; eauto. invertHyp. 
-    eapply rewindDiffStamp; eauto. eapply rewindValidPortion; eauto. }
-   {inv H5; decompSame; try invertEq. 
-    {invertEq. repeat lookupSame. omega. }
-    {invertEq. repeat lookupSame.
-     assert(validate S (readItem l E v0::L) H C (abort e' L')). inv H2. 
-     eapply validateAbortPropogate; eauto. eapply validateAbortRead; eauto. 
-     econstructor. split. eapply p_multi_step. eapply p_abortStep. 
-     eapply abortReplay; eauto. rewrite plus_comm. constructor. repeat constructor. 
-     inv H6. rewrite <- rewindIFFReplay. copy H7. 
-     eapply validateValidate in H3. invertHyp. eapply rewindDiffStamp; eauto.
-     eapply rewindValidPortion. eauto. eapply abortReplay in H7. eauto. 
-     inv H2. eapply validateAbortPropogate; eauto. eapply validateAbortRead; eauto. }
-    {invertEq. repeat lookupSame. }
-   }
-  }
-  {inv H1. inv H4. eapply replayInvalid in H8; eauto. invertHyp. 
-   econstructor. split. econstructor. eapply p_abortStep; eauto. constructor. 
-   constructor. constructor. inv H2. eapply rewindValidPortion in H5; eauto.
-   eapply validateValidate in H3. invertHyp. eapply rewindDiffStamp in H5; eauto. 
-   rewrite <- rewindIFFReplay. auto. }
-  {inv H2. inv H5. econstructor. split. econstructor.
-   eapply p_allocStep; eauto. constructor. repeat constructor. }
-  {inv H2. inv H5. inv H9. 
-   {econstructor. split. econstructor. eapply p_commitStep; eauto. 
-    constructor. repeat constructor. }
-   {inv H2; try solve[decompSame; solveByInv]. }
-  }
-  {inv H1. inv H4. econstructor. split. econstructor. 
-   eapply p_atomicStep; eauto. constructor. constructor. 
-   eapply inTXAheadOf. constructor. }
-  {inv H1. inv H4. econstructor. split. eapply p_multi_step. 
-   eapply p_betaStep; eauto. constructor. repeat constructor. }
+  {constructor; eauto. }
 Qed. 
 
+Theorem AheadOfCommitNI : forall T' C H T HV L,
+    validate L H (commit HV) ->
+    poolAheadOf H C T T' -> poolAheadOf HV (1+C) T T'. 
+Proof.
+  intros. induction H1.
+  {constructor. inv H1.
+   {constructor. }
+   {constructor. erewrite <- rewindIFFReplay in *.
+    eapply rewindCommitSingleNI; eauto. }
+  }
+  {econstructor; eauto. }
+Qed. 
+
+Theorem AheadOfNI : forall C H T C' H' T' T2 T2',
+    poolAheadOf H C T2 T2' -> f_step C H T C' H' T' ->
+    poolAheadOf H' C' T2 T2'.
+Proof.
+  intros. genDeps{{T2; T2'}}. induction H1; intros; auto. 
+  {inv H0. auto. }
+  {eapply AheadOfAlloc; eauto. }
+  {eapply AheadOfCommitNI; eauto. }
+Qed. 
+
+Ltac invertHyp := 
+  match goal with
+    |H : poolAheadOf ?h ?c (Single (Some ?tx, ?L, ?e)) ?T |- _ => inv H; try invertHyp 
+    |H : AheadOf ?h ?C (Some ?tx, ?L, ?e) ?T |- _ => inv H; try invertHyp
+    |H : poolRewind ?C ?h (Single (Some ?tx, ?L, ?e)) |- _ => inv H; try invertHyp
+    |H : poolAheadOf ?h ?C (Single(None, ?L,?e)) ?T |- _ => inv H; try invertHyp
+    |H : AheadOf ?h ?C (None, ?L, ?e) ?T |- _ => inv H; try invertHyp
+    |H : poolRewind ?C ?h (Single (None, ?L, ?t)) |- _ => inv H; try invertHyp
+    | _ => tactics.invertHyp
+  end. 
+
+Theorem valueDecidable : forall (v1 v2 : term), v1 = v2 \/ v1 <> v2.
+Proof.
+  induction v1; intros; destruct v2; try solve[right; intro; solveByInv].
+  {specialize (IHv1 v2); inv IHv1; auto; right; intro; invertEq; auto. }
+  {destruct (Nat.eq_dec n n0). subst; auto. right. intro. invertEq. auto. }
+  {left; auto. }
+  {destruct (Nat.eq_dec n n0). subst; auto. right. intro. invertEq. auto. }
+  {specialize (IHv1_1 v2_1). specialize (IHv1_2 v2_2). 
+   inv IHv1_1; inv IHv1_2; auto; right; intro; invertEq; auto. }
+  {specialize (IHv1 v2); inv IHv1; auto; right; intro; invertEq; auto. }
+  {specialize (IHv1_1 v2_1). specialize (IHv1_2 v2_2). 
+   inv IHv1_1; inv IHv1_2; auto; right; intro; invertEq; auto. }
+  {specialize (IHv1 v2); inv IHv1; auto; right; intro; invertEq; auto. }
+  {specialize (IHv1 v2); inv IHv1; auto; right; intro; invertEq; auto. }
+  {specialize (IHv1 v2); inv IHv1; auto; right; intro; invertEq; auto. }
+  {specialize (IHv1 v2); inv IHv1; auto; right; intro; invertEq; auto. }
+Qed. 
+
+
+Theorem replayAbort : forall H C S e0 L e L' e' L'' e'',
+    replay H C (Some(S, e0), L, e) (Some(S, e0), L', e') ->
+    validate L H (abort e'' L'') ->
+    validate L' H (abort e'' L'').
+Proof.
+  intros. genDeps{{e''; L''}}. dependent induction H0; intros.
+  {auto. }
+  {inv H0; eauto.
+   {eapply IHreplay. eauto. eauto. constructor; eauto. }
+   {eapply IHreplay. eauto. eauto. constructor; eauto. }
+   {eapply IHreplay. eauto. eauto. constructor; eauto. }
+  }
+Qed. 
+    
+Theorem replayValidate : forall H C S e0 L L' e e' HV,
+    replay H C (Some(S, e0), L, e) (Some(S, e0), L', e') ->
+    validate L H (commit HV) ->
+    (exists HV', validate L' H (commit HV')) \/
+    (exists L'' e'', validate L' H (abort e'' L'')). 
+Proof.
+  intros. generalize dependent HV. dependent induction H0; intros; eauto.  
+  inv H0; eauto. 
+  {assert((Some (S, e0), readItem l E v :: L, fill E v) ~= (Some (S, e0), readItem l E v :: L, fill E v)).
+   auto. eapply IHreplay in H0; auto. inv H0; invertHyp; eauto.
+   econstructor; eauto. }
+  {destruct (valueDecidable v v'). 
+   {assert((Some (S, e0), readItem l E v' :: L, fill E v') ~= (Some (S, e0), readItem l E v' :: L, fill E v')).
+    auto. subst. eapply IHreplay in H3; eauto. constructor; eauto. }
+   {right. exists L. exists (fill E (get (loc l))). eapply replayAbort; eauto.
+    eapply validateAbortRead; eauto. }
+  }
+  {assert((Some (S, e0), writeItem l v :: L, fill E unit) ~= (Some (S, e0), writeItem l v :: L, fill E unit)).
+   auto. eapply IHreplay in H0; eauto. econstructor; eauto. }
+Qed. 
+
+    
+    
+Theorem validateDeterministic : forall L H res res',
+    validate L H res -> validate L H res' -> res = res'.
+Proof.
+  intros. generalize dependent res'. induction H0; intros.  
+  {inv H1. auto. }
+  {inv H2; eauto. transEq. invertEq. exfalso; auto. }
+  {inv H1; eauto. eapply IHvalidate in H5. solveByInv.
+   eapply IHvalidate in H7. solveByInv. }
+  {inv H3; eauto. transEq. invertEq. exfalso; auto.
+   eapply IHvalidate in H9. solveByInv. }
+  {inv H1; eauto. eapply IHvalidate in H7; solveByInv.
+   eapply IHvalidate in H8. invertEq. auto. }
+Qed. 
+   
+Theorem tsExtendCatchUp : forall H C S L e e0 L' e' L'' e'' HV,
+    validate L' H (abort e'' L'') -> validate L H (commit HV) -> 
+    rewind H C (Some(S, e0), L, e) (Some(S, e0), L', e') ->
+    rewind H C (Some(S, e0), L, e) (Some(S, e0), L'', e'').
+Proof.
+  intros. genDeps{{L''; e''}}. dependent induction H2; intros.
+  {eapply validateDeterministic in H1; eauto. solveByInv. }
+  {inv H3; eauto. 
+   {inv H0; eauto. eapply decomposeEq in H10.
+    subst. assumption. }
+   {inv H0; eauto. eapply decomposeEq in H11. subst. eauto. }
+   {inv H0. eauto. }
+  }
+Qed. 
+
+(*partial abort can simulate full abort*)
+Theorem fullImpliesPartial : forall C H T C' H' T' PT, 
+    f_step C H T C' H' T' -> poolAheadOf H C T PT ->
+    poolRewind C H PT -> 
+    exists PT', p_multistep C H PT C' H' PT' /\
+           poolAheadOf H' C' T' PT'.
+Proof.
+  intros. generalize dependent PT. induction H0; intros.
+  {inv H0. invertHyp. copy H7. eapply replayInvalid in H7; eauto. invertHyp. 
+   econstructor. split. eapply c_multi_step. eapply c_liftedStep. 
+   econstructor. eauto. constructor. econstructor. econstructor. 
+   copy H2. eapply rewindAbort in H2; eauto.
+   eapply validateValidate in H0; eauto. invertHyp. 
+   rewrite <- rewindIFFReplay. eapply rewindNewerStamp; eauto. }
+  {inv H0; try invertHyp. 
+   {inv H10. 
+    {econstructor. split. eapply c_multi_step. eapply c_transStep. 
+     econstructor; eauto. constructor. repeat econstructor. }
+    {econstructor. split. constructor. constructor. constructor.  
+     inv H0; try decompSame; invertEq. repeat transEq. invertEq.
+     eauto. omega. transEq. invertEq. }
+   }
+   {inv H9.
+    {econstructor. split. eapply c_multi_step. eapply c_transStep.
+     econstructor; eauto. constructor. repeat econstructor. }
+    {econstructor. split. repeat constructor. repeat constructor. 
+     inv H0; try decompSame; invertEq. transEq. invertEq.
+     repeat transEq. invertEq. transEq. invertEq. auto. }
+   }
+   {destruct S. Focus 2. exfalso; auto. invertHyp. inv H8.
+    {econstructor. split. eapply c_multi_step. eapply c_transStep.
+     eapply t_writeStep; eauto. constructor. repeat constructor. }
+    {econstructor. split. repeat constructor. repeat constructor.
+     inv H0; try decompSame; invertEq. assumption. }
+   }
+   {destruct S. Focus 2. exfalso; auto. invertHyp. inv H8.
+    {econstructor. split. eapply c_multi_step. eapply c_transStep.
+     eapply t_atomicIdemStep; eauto. constructor. repeat constructor. }
+    {econstructor. split. repeat constructor. repeat constructor.
+     inv H0; try decompSame; invertEq. assumption. }
+   }
+   {destruct S. Focus 2. exfalso; auto. invertHyp. inv H8.
+    {econstructor. split. eapply c_multi_step. eapply c_transStep.
+     eapply t_betaStep; eauto. constructor. repeat constructor. }
+    {econstructor. split. repeat constructor. repeat constructor.
+     inv H0; try decompSame; invertEq. assumption. }
+   }
+  }
+  {inv H1. inv H2. eapply IHc_step in H5; auto. invertHyp. econstructor.
+   split. eapply c_multi_L. eassumption. constructor. auto.
+   eapply AheadOfNI; eauto. }
+  {inv H1. inv H2. eapply IHc_step in H7; auto. invertHyp. econstructor.
+   split. eapply c_multi_R. eassumption. constructor.
+   eapply AheadOfNI; eauto. auto. }
+  {invertHyp.  econstructor. split. eapply c_multi_step.
+   eapply c_forkStep; eauto. constructor. repeat econstructor. }
+  {invertHyp. econstructor. split. eapply c_multi_step.
+   eapply c_allocStep; eauto. constructor. repeat econstructor. }
+  {invertHyp. inv H9.
+   {econstructor. split. eapply c_multi_step. eapply c_commitStep; eauto.
+    constructor. repeat constructor. }
+   {inv H2; decompSame; invertEq. }
+  }
+  {invertHyp. econstructor. split. eapply c_multi_step.
+   eapply c_atomicStep; eauto. constructor. repeat econstructor. }
+  {invertHyp. econstructor. split. eapply c_multi_step.
+   eapply c_betaStep; eauto. constructor. repeat econstructor. }
+  {invertHyp. copy H8. eapply replayValidate in H8; eauto. inv H8.
+   {invertHyp. econstructor. split. eapply c_multi_step. eapply c_tsExtend.
+    eauto. constructor. repeat constructor. rewrite <- rewindIFFReplay in *.
+    eapply rewindNewerStamp; eauto. }
+   {invertHyp. econstructor. split. eapply c_multi_step. eapply c_liftedStep.
+    econstructor; eauto. constructor. repeat constructor.
+    erewrite <- rewindIFFReplay in *. copy H2. eapply validateValidate in H2.
+    invertHyp. eapply rewindNewerStamp; eauto.
+    eapply tsExtendCatchUp; eauto. }
+  }
+Qed. 
+
+   
 (*generalize step preserves rewind to thread pools*)
 Theorem multistepPreservesRewind : forall C H T C' H' T',
                                 poolRewind C H T -> p_multistep C H T C' H' T' ->
                                 poolRewind C' H' T'. 
 Proof.
-  intros. induction H1. auto. apply IHp_multistep.
+  intros. induction H1. auto. apply IHc_multistep.
   eapply p_stepRewind; eauto. 
 Qed. 
 
 (*generalize full implies partial to thread pools*)
 Theorem fullImpliesPartialMulti : forall C H T C' H' T' PT, 
-                               f_multistep C H T C' H' T' -> poolAheadOf H T PT ->
+                               f_multistep C H T C' H' T' -> poolAheadOf H C T PT ->
                                poolRewind C H PT ->
                                exists PT', p_multistep C H PT C' H' PT' /\
-                                           poolAheadOf H' T' PT'.
+                                           poolAheadOf H' C' T' PT'.
 Proof.
   intros. generalize dependent PT. induction H0; intros. 
   {exists PT. split. constructor. auto. }
   {copy H0. eapply fullImpliesPartial in H0; eauto. invertHyp. 
    copy H0. apply multistepPreservesRewind in H5; auto. 
-   eapply IHf_multistep in H6; eauto. invertHyp. exists x0. split. 
-   eapply p_multi_trans; eauto. auto. }
+   eapply IHc_multistep in H6; eauto. invertHyp. exists x0. split. 
+   eapply c_multi_trans; eauto. auto. }
 Qed. 
 
 
